:recycle: reorganize parts

lecture2/parts/1-intro.dfy
@@ -58,102 +58,31 @@ lemma AbsCorrect(x: int) {
 }
 
 /*
+Recap:
+
+- We wrote a program & proved it correct (in the same framework)
+
+- abs() is **both** an executable function and mathematically understandable (verifiable) code
 
 Poll:
-Which of the following are most likely to be useful steps for verification of a real-world software project?
 
-https://forms.gle/fHwrbRw6JGfscLab9
 
 =====
 
-So far, we could do all of this with just validity. (Why?)
-
-Q: Are there things we can't express using only validity?
-
-Yes: for example, abs() is surjective onto nonnegative integers:
 */
-
-predicate is_nonnegative(y: int) {
-    y >= 0
-}
-
-lemma AbsSurjective()
-ensures forall y: int :: is_nonnegative(y) ==> exists x :: abs(x) == y
-{
-    // Some odd syntax
-    // Commenting the below out - Dafny cannot prove this
-    // We need to help Dafny out by providing the proof.
-    forall y: int | is_nonnegative(y)
-    ensures exists x :: abs(x) == y
-    {
-        AbsSurjectiveFor(y);
-    }
-}
-
-lemma AbsSurjectiveFor(y: int)
-requires y >= 0
-ensures exists x :: abs(x) == y
-{
-    assert abs(y) == y;
-    // asserts abs(-y) == y; // also works
-}
 
 /*
-    Eventually, it will become clear that we can also verify arbitrary programs
-    and this verification will be built on first-order logic.
+    === Method/function distinction ===
 
-    Here's a small sneak peak:
+    The main difference between methods and functions is that
+    methods need pre/postconditions to work, functions don't need
+    pre/postconditions and are purely mathematical functions.
+    function = mathematical function
+    method = imperative code, i.e. Python/C/C++ function
 
-    Below, we wrote a function to add up the absolute value sum of a list, like
-
-    AbsSum([x, y, z]) = abs(x) + abs(y) + abs(z).
-
-    The spec here says that AbsSum is an upper bound on all individual elements of the list.
 */
 
-method AbsSum(l: seq<int>) returns (result: int)
-ensures
-    forall i :: 0 <= i < |l| ==> result >= abs(l[i])
-{
-    var sum: nat := 0;
-    for j := 0 to |l|
-    // While loop version:
-    // var j := 0;
-    // while j < |l|
-        // Unfamiliar concept: loop invariant
-        // Think of this as pre and postconditions on the loop. We will
-        // see more on this later.
-        // Note: the following line would be needed for a while loop,
-        // added implicitly for a for loop.
-        // invariant j <= |l|
-        invariant forall i :: 0 <= i < j ==> sum >= abs(l[i])
-    {
-        sum := sum + abs(l[j]);
-        // While loop version:
-        // j := j + 1;
-    }
-    result := sum;
-    // equiv. syntax:
-    // return sum;
-}
-
-/*
-    Above: we have a program and we have proved it correct!
-
-    Let's see how this is accomplished by starting with some mini verification
-    exercises.
-
-    After this I want to go deeper to understand on a fundamental level:
-    - What is a proof?
-    - What is a program?
-*/
-
-// Note: alternate way of writing Abs as a method.
-// The main difference between methods and functions is that
-// methods need pre/postconditions to work, functions don't need
-// pre/postconditions and are purely mathematical functions.
-//    function = mathematical function
-//    method = imperative code, i.e. Python/C/C++ function
+// Below: alternate way of writing Abs as a method.
 method AbsMethod(x: int) returns (y: int)
     ensures y >= 0
     ensures y == x || y == -x
@@ -166,64 +95,22 @@ method AbsMethod(x: int) returns (y: int)
 }
 
 /*
+    Preconditions and postconditions
+
+    Using a method means we can directly specify pre/posts on
+    the method:
+
+        requires = precondition
+
+        ensures = postcondition
+
+    Exercise:
+
+    Add a precondition to the above
+    and strengthen the postcondition
+*/
 
 /*
-    === Recap ===
+=== Recap ===
 
-    We saw some examples of writing
-    functions, assertions, lemmas, and postconditions in Dafny.
-    (The postconditions are the "ensures" statements.)
-    We also saw examples of quantifiers.
-
-    forall x :: formula
-    exists x :: formula
-
-    ===== A note on industry applications =====
-
-    Course goals:
-    - to understand how verification works
-    - to apply verification to real-word projects
-
-    The methodology of verification:
-
-    1. We encode the problem we are considering
-      (based on real software, in a real industry application)
-      in preconditions, postconditions, and other domain-specific constraints
-      in an appropriate verification framework.
-
-    2. We use the tool to prove the property, thus proving the code 100% free from bugs.
-
-    When is this methodology useful in practice?
-    Not always! But often in cases where correctness, safey, or security is critical
-    to system functioning.
-    Investment examples:
-
-    - Amazon: verifying low-level cryptographic libraries using tools
-      like Dafny and CBMC, verifying domain-specific security constraints
-      (e.g., your cloud data cannot be accessed by untrusted users)
-
-    - Microsoft: many applications of Z3 and other techniques internally, verifying network code,
-      device and kernel drivers, etc.
-
-    - Hardware bugs & hardware verification:
-
-        Pentium FDIV bug: affected Intel Pentium processors in 1994.
-        recall of all defective Intel processors at the time
-        $475 million in losses!
-
-    - Signal messaging app: verification effort for core messaging protocol going back to 2017
-
-    - Larger-scale realistic software projects coming from academia:
-        CompCert: a verified optimizing C compiler
-        CertiKOS: a verified operating system kernel
-        Increasing interest from the systems community and more work every year on building
-        bigger verified file systems, network controllers, etc.
-
-    - More generally, at large industry scale, security bugs cost a LOT of money.
-      Higher-ups will throw money at any technique which even has a chance of preventing large-scale
-      security risks (willing to invest).
-
-    - The argument is that despite a much greater effort, we also get a greater payoff.
-      Verify your library ==> greater assurance against threats, more people want to use it,
-      maintain the verification conditions on all future software updates
 /*
