lecture2/parts/2-methodology-filled.dfy
@@ -1,0 +1,131 @@
+/*
+Lecture 2, Part 2:
+Verification methodology.
+
+This is a filled version of the 2-methodology.dfy file.
+
+We will fill out the file in class.
+*/
+
+/*
+    Exercise 1:
+    Write a function to compute the minimum of four integers.
+*/
+
+method MinFour(a: int, b: int, c: int, d: int) returns (result: int)
+// Spec:
+// requires true // no precondition
+// requires false
+ensures result <= a && result <= b && result <= c && result <= d
+ensures result == a || result == b || result == c || result == d
+{
+    if a <= b && a <= c && a <= d {
+        return a;
+        // Equiv. syntax:
+        // result := a;
+        // return;
+    }
+    if b <= c && b <= d {
+        return b;
+    }
+    if c <= d {
+        return c;
+    }
+    return d;
+}
+
+/*
+    Exercise 2:
+    Write a function to compute the *argument minimum* of four integers.
+
+    Note: the "argument min" is the index of the smallest integer.
+
+    Let's say:
+    index of a is 0, b is 1, c is 2, and d is 3.
+
+    Start by writing the imperative code
+*/
+
+method ArgMinFour(a: int, b: int, c: int, d: int) returns (result: int)
+// What should the spec be?
+// requires a != b && a != c && a != d && b != c && b != d && c != d
+// ensures (result == 0 && a <= b && a <= c && a <= d)
+//     || (result == 1 && b <= a && b <= a && b <= d)
+//     || (result == 2 && c <= a && c <= b && c <= d)
+//     || (result == 3 && d <= a && d <= b && d <= c)
+ensures 0 <= result <= 3
+ensures result == 0 ==> (a <= b && a <= c && a <= d)
+ensures result == 1 ==> (b <= a && b <= c && b <= d)
+ensures result == 2 ==> (c <= a && c <= b && c <= d)
+ensures result == 3 ==> (d <= a && d <= b && d <= c)
+// Note: cannot do a == MinFour(a, b, c, d)
+// b.c. cannot call method in a formula/expression context.
+// requires ...
+// ensures ...
+// Note: one way to mark a function as unimplemented:
+{
+    // Impl. 1: via direct comparison
+    // if a <= b && a <= c && a <= d {
+    //     return 0;
+    // }
+    // if b <= c && b <= d {
+    //     return 1;
+    // }
+    // if c <= d {
+    //     return 2;
+    // }
+    // return 3;
+
+    // Or we could use the previous function...
+    // Impl 2.: using the previous function
+    var y := MinFour(a, b, c, d);
+    if y == a {
+        return 0;
+    } else if y == b {
+        return 1;
+    } else if y == c {
+        return 2;
+    } else if y == d {
+        return 3;
+    } else {
+        // This branch is unreachable
+        assert false;
+    }
+}
+
+/*
+    Exercise 3:
+    Write unit tests for the above.
+*/
+
+method TestMin() {
+    var result1 := MinFour(1, 2, 3, 4);
+    assert result1 == 1;
+    var result2 := MinFour(3, 3, 3, 4);
+    assert result2 == 3;
+}
+
+method TestArgMin() {
+    var result1 := ArgMinFour(1, 2, 3, 4);
+    assert result1 == 0;
+    var result2 := ArgMinFour(3, 3, 3, 4);
+    assert result2 == 0 || result2 == 1 || result2 == 2;
+}
+
+// Summary: There were 3 possible design choices for ArgMin:
+// - Leave the behavior underspecified; has to return one min index, any is OK on tie
+// - Exclude the behavior by adding a precondition (require all vals are distinct)
+// - Specify the behavior in the case of ties: e.g., return the first or the last index
+//   of a min value.
+
+/*
+    Additional exercises
+    (Optional or skip for time)
+
+    Exercise 7
+    Let's try to write a verified version of the
+    four-numbers problem solver from HW1.
+
+    Full disclosure: I didn't have a chance to try this offline.
+    It is possible, but may be fairly difficult.
+*/
