lecture2/parts/3-quantifiers.dfy
@@ -1,0 +1,125 @@
+/*
+    Lecture 2, part 2:
+    Quantifiers
+
+So far, we think of
+
+    verification = prove the spec true on all inputs
+
+Q: Are there things we can't express this way?
+
+A: Yes: for example, abs() is surjective onto nonnegative integers:
+*/
+
+function abs(x: int): int {
+    if x > 0 then x else -x
+}
+
+predicate is_nonnegative(y: int) {
+    y >= 0
+}
+
+lemma AbsSurjective()
+ensures forall y: int :: is_nonnegative(y) ==> exists x :: abs(x) == y
+{
+    // Some odd syntax
+    // Commenting the below out - Dafny cannot prove this
+    // We need to help Dafny out by providing the proof.
+    forall y: int | is_nonnegative(y)
+    ensures exists x :: abs(x) == y
+    {
+        AbsSurjectiveFor(y);
+    }
+}
+
+lemma AbsSurjectiveFor(y: int)
+requires y >= 0
+ensures exists x :: abs(x) == y
+{
+    assert abs(y) == y;
+    // asserts abs(-y) == y; // also works
+}
+
+/*
+    Eventually, it will become clear that we can also verify arbitrary programs
+    and this verification will be built on first-order logic.
+
+    Here's a small sneak peak:
+
+    Below, we wrote a function to add up the absolute value sum of a list, like
+
+    AbsSum([x, y, z]) = abs(x) + abs(y) + abs(z).
+
+    The spec here says that AbsSum is an upper bound on all individual elements of the list.
+*/
+
+method AbsSum(l: seq<int>) returns (result: int)
+ensures
+    forall i :: 0 <= i < |l| ==> result >= abs(l[i])
+{
+    var sum: nat := 0;
+    for j := 0 to |l|
+    // While loop version:
+    // var j := 0;
+    // while j < |l|
+        // Unfamiliar concept: loop invariant
+        // Think of this as pre and postconditions on the loop. We will
+        // see more on this later.
+        // Note: the following line would be needed for a while loop,
+        // added implicitly for a for loop.
+        // invariant j <= |l|
+        invariant forall i :: 0 <= i < j ==> sum >= abs(l[i])
+    {
+        sum := sum + abs(l[j]);
+        // While loop version:
+        // j := j + 1;
+    }
+    result := sum;
+    // equiv. syntax:
+    // return sum;
+}
+
+/*
+    We can also rewrite our specs for abs ...
+*/
+
+// Another way of writing...
+lemma AbsCorrectQuantifiers() {
+    assert forall x :: abs(x) >= 0;
+    assert forall x :: abs(x) == x || abs(x) == -x;
+    // ^^ quantifiers!
+    //    this takes us away from quantifier-free logics to "first-order logic" (FOL).
+    // Try modifying this.
+
+    // What about this?
+    // assert exists x :: abs(x) == 1;
+    // No proof! More on this soon.
+
+    // Sadly quantifiers are hard! So we have to help Dafny out sometimes.
+    // We will need to get our hands dirty with the proofs.
+}
+
+// Another way of writing the correctness spec for Abs
+lemma AbsCorrect2()
+// ensures = a postcondition
+ensures forall x :: abs(x) >= x
+ensures forall x :: abs(x) == x || abs(x) == -x
+{}
+
+/*
+    Why do we need quantifiers?
+
+    Another example using abs():
+    Suppose we want to show that abs() is increasing:
+
+        forall x. forall y. 0 <= x < y ==> abs(x) < abs(y)
+
+    Only forall statements in front! So we can do this with a validity check:
+*/
+
+lemma AbsIncreasing()
+ensures
+    forall x :: forall y :: 0 <= x < y ==> abs(x) <= abs(y)
+{
+    // Proof goes through - QED
+}
