lecture2/parts/4-loop-invariants.dfy
@@ -1,0 +1,176 @@
+/*
+Lecture 2, Part 4:
+Loop invariants
+
+Recap:
+We have seen:
+
+- How to write Dafny code with preconditions and postconditions
+- Writing assertions, lemmas, and unit tests
+- Function/method distinction
+
+The MinFour and ArgMinFour were a bit artificial as they only work with integers.
+It would be nice to generalize our functions to work with lists!
+Can we?
+This requires: loop invariants!
+
+Continuing the 3-step process:
+1. Decide on an implementation (or port an existing one); write in Dafny
+2. Decide on a spec; write pre/postconditions
+3. Help Dafny with the proof (as needed)
+
+We did step 1, now step 2:
+
+=== Poll ===
+
+Write a precondition and postcondition for MinList
+that matches what we had for MinFour.
+(Your pre and postcondition don't have to be valid Dafny, but they should be
+ correct logically)
+*/
+
+/*
+    Exercise:
+    Generalize the MinFour implementation and specs
+    to lists of integers, rather than just four.
+
+    Two "list"-y types in Dafny: array and seq
+
+    List syntax:
+    array<int>
+    a.Length
+    a[i]
+
+    Pseudocode:
+    Keep track of a minimum value
+    Iterate through the array, update the min when a smaller value is encountered
+*/
+
+/*
+=== What is a loop invariant? ===
+
+A loop invariant is like a pre/postcondition for the loop body.
+
+A loop invariant must satisfy the following 3 conditions:
+1. Loop invariant is true before first entering the loop
+    precondition ==> invariant
+
+2. If the loop condition is true, then the loop invariant is preserved
+    (loop condition) && invariant holds at the start ===> invariant holds at end
+
+3. If the loop condition is false, then the loop invariant implies the postcondition
+    !(loop condition) && invariant holds ==> postcondition.
+
+*/
+
+method MinList(a: array<int>) returns (result: int)
+// Precondition: array is nonempty
+requires a.Length > 0
+// Postcondition: for all i between 0 and the length, the result should be <= a[i]
+// and, there exists an i between 0 and the length, such that the result is == a[i].
+ensures forall i :: 0 <= i < a.Length ==> result <= a[i]
+ensures exists i :: 0 <= i < a.Length && result == a[i]
+{
+    var min := a[0];
+    // invariant should be true here
+    for i := 0 to a.Length
+    invariant forall j :: 0 <= j < i ==> min <= a[j]
+    invariant 0 <= i <= a.Length // implicitly added for for loops - so not technically needed.
+    // Option 1:
+    invariant i == 0 ==> min == a[0]
+    invariant i >= 1 ==> exists j :: 0 <= j < i && min == a[j]
+    // Option 2:
+    // invariant exists j :: 0 <= j < a.Length && min == a[j]
+    {
+        if a[i] < min {
+            min := a[i];
+        }
+
+        // implicit: at the end of each loop, we do i := i + 1
+
+        // invariant should be true here
+        // what is true about the array and the variables min, i at this point in the program?
+        // min <= a[0]
+        // min <= a[0], a[1], ..., a[i-1]
+        // i is between 0 and a.Length -- 0 <= i < a.Length
+        // min is an element of the array that we've looked at so far: min == a[0], a[1], ..., a[i-1].
+    }
+    return min;
+}
+
+method ArgMinList(a: array<int>) returns (result: int)
+requires a.Length > 0
+// What to do about ties?
+// In the case of ties: return the first index.
+ensures 0 <= result < a.Length
+ensures forall i :: 0 <= i < a.Length ==> a[result] <= a[i]
+ensures forall i :: 0 <= i < result ==> a[result] < a[i]
+{
+    var min := a[0];
+    var min_index := 0;
+    for i := 1 to a.Length
+    invariant 0 <= min_index < i
+    // proof also goes through with the weaker: 0 <= min_index < a.Length.
+    invariant min == a[min_index]
+    invariant forall j :: 0 <= j < min_index ==> min < a[j]
+    invariant forall j :: 0 <= j < i ==> min <= a[j]
+    {
+        if a[i] < min {
+            min := a[i];
+            min_index := i;
+        }
+    }
+    result := min_index;
+}
+
+/*
+    Additional practice with loop invariants:
+
+    Exercise 5:
+    (Skip for time)
+    Write a function to compute the gcd of two integers.
+*/
+
+/*
+    Exercise 6
+    Write a unit test for the ArgMinList and MinList functions.
+
+    (Compile time unit test - checked at compile time, not executed)
+
+    What happens?
+    This will lead to a topic that we will discuss next.
+*/
+
+method TestMinList() {
+    var a0 := new int[][1]; // new keyword: allocates an array on the heap
+    var y0 := MinList(a0);
+    assert y0 == 1;
+    var a1 := new int[][1, 0, 1];
+    var y1 := MinList(a1);
+    // Helping Dafny out...
+    // assert forall i :: 0 <= i < a1.Length ==> y1 <= a1[i];
+    // assert exists i :: 0 <= i < a1.Length && y1 == a1[i];
+    // assert a1.Length == 3;
+    // assert forall i :: 0 <= i < 3 ==> y1 <= a1[i];
+    // assert exists i :: 0 <= i < 3 && y1 == a1[i];
+    // assert y1 <= a1[0];
+    assert y1 <= a1[1];
+    // assert y1 <= a1[2];
+    // assert y1 <= 0;
+
+    assert y1 == 0;
+    // var a2 := new int[][5, 4, 3, 2, 1];
+    // var y2 := MinList(a2);
+    // assert ...
+}
+
+/*
+    Recap
+
+    - We saw examples of working with arrays: a[i], a.Length etc.
+    - We defined loop invariants and saw them in actino
+    - We discussed the computationally bounded nature of Dafny, and how
+      when writing unit tests we may need additional assertions to walk through
+      and help Dafny prove the assertion
+    - This is a more general debugging technique: find out what Dafny knows, and what it doesn't.
+*/
