lecture2/parts/5-conclusions.dfy
@@ -1,0 +1,79 @@
+/*
+Lecture 2, Part 5:
+Conclusions
+
+=== Poll (to wrap up this section) ===
+
+Consider the following snippet of a program:
+
+assert P;
+assert Q;
+
+Suppose that P implies Q (logically) but Dafny verification passes only for P, and not Q. Which of the following is a possible reason for this? (Select all that apply)
+
+=== End notes ===
+
+What are the main limitations of Dafny?
+
+1. High effort to write and verify real-world software
+2. Q is true, but not provable from P?
+
+(1) is true, but not fundamental.
+(2) is actually possible and is more fundamental.
+
+To understand the more fundamental limits of Dafny,
+then, we need to go back to the logics on which Dafny is built,
+and in particular to proofs in first-order logic (FOL).
+See the file fol.dfy.
+*/
+
+/*
+    ===== A note on industry applications =====
+
+    Course goals:
+    - to understand how verification works
+    - to apply verification to real-word projects
+
+    The methodology of verification:
+
+    1. We encode the problem we are considering
+      (based on real software, in a real industry application)
+      in preconditions, postconditions, and other domain-specific constraints
+      in an appropriate verification framework.
+
+    2. We use the tool to prove the property, thus proving the code 100% free from bugs.
+
+    When is this methodology useful in practice?
+    Not always! But often in cases where correctness, safey, or security is critical
+    to system functioning.
+    Investment examples:
+
+    - Amazon: verifying low-level cryptographic libraries using tools
+      like Dafny and CBMC, verifying domain-specific security constraints
+      (e.g., your cloud data cannot be accessed by untrusted users)
+
+    - Microsoft: many applications of Z3 and other techniques internally, verifying network code,
+      device and kernel drivers, etc.
+
+    - Hardware bugs & hardware verification:
+
+        Pentium FDIV bug: affected Intel Pentium processors in 1994.
+        recall of all defective Intel processors at the time
+        $475 million in losses!
+
+    - Signal messaging app: verification effort for core messaging protocol going back to 2017
+
+    - Larger-scale realistic software projects coming from academia:
+        CompCert: a verified optimizing C compiler
+        CertiKOS: a verified operating system kernel
+        Increasing interest from the systems community and more work every year on building
+        bigger verified file systems, network controllers, etc.
+
+    - More generally, at large industry scale, security bugs cost a LOT of money.
+      Higher-ups will throw money at any technique which even has a chance of preventing large-scale
+      security risks (willing to invest).
+
+    - The argument is that despite a much greater effort, we also get a greater payoff.
+      Verify your library ==> greater assurance against threats, more people want to use it,
+      maintain the verification conditions on all future software updates
+*/
